Chen/Unproductive.thy
@@ -9,38 +9,76 @@ hide_const (open) Topological_Spaces.closed
 
 text \<open>Unproductive Symbol Elimination\<close>
 
-definition "rm_unproductive P = {(A,\<alpha>) |A \<alpha>. (A,\<alpha>) \<in> P \<and> Lang P A \<noteq> {}}"
+(* I think the inductive set definition is better, because we may want to use
+producthive.induct at some point *)
+inductive_set productive :: "('n,'t)Prods \<Rightarrow> 'n set" for P where
+"\<lbrakk> (A,\<alpha>) \<in> P; \<And>B. B \<in> nts_of_syms \<alpha> \<Longrightarrow> B \<in> productive P \<rbrakk> \<Longrightarrow> A \<in> productive P"
+print_theorems
 
-
-lemma prefix_rm_unproductive: "rm_unproductive P \<subseteq> P"
-  unfolding rm_unproductive_def by auto
-
-lemma derivs_if_derives_unproductive: "P \<turnstile> \<alpha> \<Rightarrow>* \<beta> \<Longrightarrow> rm_unproductive P \<turnstile> \<alpha> \<Rightarrow>* \<beta>"
-proof (induction rule: rtrancl_derive_induct)
-  case base
-  then show ?case by simp
-next
-  case (step u A v w)
-  then show ?case
-    oops
+definition "rm_unproductive P = {(A,\<alpha>) \<in> P. A \<in> productive P}"
 
 
 theorem "Lang (rm_unproductive P) A = Lang P A"
   proof
-    show "Lang (rm_unproductive P) A \<subseteq> Lang P A"
-      using prefix_rm_unproductive Lang_mono by metis
+    have "rm_unproductive P \<subseteq> P"
+      unfolding rm_unproductive_def by auto
+    then show "Lang (rm_unproductive P) A \<subseteq> Lang P A"
+      using Lang_mono by metis
   next
-    consider (LangEmpty) "Lang P A = {}" | (NotLangEmpty) "Lang P A \<noteq> {}"
-      by auto
-    then show "Lang P A \<subseteq> Lang (rm_unproductive P) A"
-    proof (cases)
-      case LangEmpty
-      then show ?thesis by simp
-    next
-      case NotLangEmpty
-      then show ?thesis
-      unfolding rm_unproductive_def
-      sorry
+    show "Lang P A \<subseteq> Lang (rm_unproductive P) A"
+      proof (cases)
+        assume "A \<in> productive P"
+        have "\<And> w. w \<in> Lang P A \<Longrightarrow> w \<in> Lang (rm_unproductive P) A"
+          proof -
+            fix w
+            assume "w \<in> Lang P A"
+            then have "P \<turnstile> [Nt A] \<Rightarrow>* map Tm w"
+              unfolding Lang_def by simp
+            then have "rm_unproductive P \<turnstile> [Nt A] \<Rightarrow>* map Tm w"
+            sorry
+
+            then show "w \<in> Lang (rm_unproductive P) A"
+            sorry
+          qed
+        then show ?thesis
+          by auto
+      next
+        assume "A \<notin> productive P"
+        have "Lang P A = {}"
+        proof (rule ccontr)
+          assume "Lang P A \<noteq> {}"
+          then obtain w where "P \<turnstile> [Nt A] \<Rightarrow>* w" and "nts_of_syms w = {}"
+            unfolding Lang_def nts_of_syms_def by fastforce
+
+          (* should follow frow A \<notin> productive P, although I'm not sure if the 
+          current attempt at proving it is particularly fruitful*)
+          moreover have "nts_of_syms w \<noteq> {}"
+            using \<open>P \<turnstile> [Nt A] \<Rightarrow>* w\<close> unfolding nts_of_syms_def 
+            proof (induction)
+              case base
+              then show ?case by simp
+            next
+              case (step y z)
+              then obtain \<alpha> \<beta> \<gamma> A' where "y = \<alpha> @ [Nt A'] @ \<gamma>" and "z = \<alpha> @ \<beta> @ \<gamma>"
+                by (meson derive.cases)
+              (* easily proved with an additional lemma*)
+              then have "A' \<notin> productive P"
+              using \<open>A \<notin> productive P\<close> step.hyps unfolding productive_def 
+              sorry
+              show ?case
+                proof (rule ccontr)
+                  assume "\<not>({A. Nt A \<in> set z} \<noteq> {})"
+                  (* then have "y \<in> productive P" *)
+                  then show False
+                sorry
+              qed
+            qed
+          
+          ultimately show False
+            by simp
+        qed
+        then show ?thesis
+          by auto
     qed
 qed
 end
